LeanIMP/BigStep.lean
@@ -1,0 +1,77 @@
+import LeanIMP.Basic
+import LeanIMP.BigStepBasic
+import LeanIMP.IMPState
+
+open BigStep
+
+def IMPProgram.big_step_ext_eq (p1 p2 : IMPProgram) : Prop :=
+  forall (s : IMPState),
+  (forall (s_end1 : IMPState), BigStep p1 s s_end1 -> (exists s_end2 : IMPState, And (IMPState.ext_eq s_end1 s_end2) (BigStep p2 s s_end2)))
+  ∧
+  (forall (s_end2 : IMPState), BigStep p2 s s_end2 -> (exists s_end1 : IMPState, And (IMPState.ext_eq s_end2 s_end1) (BigStep p1 s s_end1)))
+
+theorem IMPProgram.big_step_ext_eq_reflexive (p : IMPProgram) : IMPProgram.big_step_ext_eq p p :=
+  by
+    intro s
+    apply And.intro
+    -- case 1
+    intros s_end1
+    intros h
+    exists s_end1
+    apply And.intro
+    exact (IMPState.ext_eq_reflexive s_end1)
+    exact h
+    -- case 2
+    intros s_end2
+    intros h
+    exists s_end2
+    apply And.intro
+    exact (IMPState.ext_eq_reflexive s_end2)
+    exact h
+
+theorem IMPProgram.big_step_ext_eq_symmetric {p1 p2 : IMPProgram} : (IMPProgram.big_step_ext_eq p1 p2) -> (IMPProgram.big_step_ext_eq p2 p1)  :=
+  by
+    unfold IMPProgram.big_step_ext_eq
+    intros h
+    intros s
+    let h_temp := h s
+    apply And.intro
+    exact h_temp.right
+    exact h_temp.left
+
+theorem IMPProgram.big_step_ext_eq_transitive {p1 p2 p3 : IMPProgram} : (IMPProgram.big_step_ext_eq p1 p2) -> (IMPProgram.big_step_ext_eq p2 p3) -> (IMPProgram.big_step_ext_eq p1 p3)  :=
+  by
+    unfold IMPProgram.big_step_ext_eq
+    intros h12 h23
+    intros s
+    apply And.intro
+    -- case 1
+    intros s_end1
+    intros h_temp
+    let h2_exists := (((h12 s).left s_end1 h_temp))
+    rcases h2_exists with ⟨w, pw⟩
+    let h2 := pw.right
+    let h3_exists := (h23 s).left w h2
+    rcases h3_exists with ⟨w2, pw2⟩
+    exists w2
+    apply And.intro
+    exact (IMPState.ext_eq_transitive pw.left pw2.left)
+    exact (pw2.right)
+    -- case 2
+    intros s_end2
+    intros h_temp
+    let h2_exists := (((h23 s).right s_end2 h_temp))
+    rcases h2_exists with ⟨w, pw⟩
+    let h2 := pw.right
+    let h1_exists := (h12 s).right w h2
+    rcases h1_exists with ⟨w2, pw2⟩
+    exists w2
+    apply And.intro
+    exact (IMPState.ext_eq_transitive pw.left pw2.left)
+    exact (pw2.right)
+
+
+instance : Equivalence IMPProgram.big_step_ext_eq where
+  refl := IMPProgram.big_step_ext_eq_reflexive
+  symm := IMPProgram.big_step_ext_eq_symmetric
+  trans := IMPProgram.big_step_ext_eq_transitive
